ok

SStructTT/SStruct/Runtime/Heap.lean
@@ -1,12 +1,33 @@
-import SStructTT.SStruct.Erasure.Syntax
+import SStructTT.SStruct.Erasure.Erased
 import Mathlib.Data.Finmap
 
 namespace SStruct.Erasure
 namespace Runtime
-variable {Srt : Type}
+variable {Srt : Type} [ord : SrtOrder Srt]
 
-abbrev Heap Srt := Finmap (fun (_ : Nat) => Tm Srt × Srt)
+inductive Cell Srt where
+  | clo (m : Tm Srt)  (s : Srt) (_ : m.NF 1)
+  | box (l : Nat)     (s : Srt)
+  | tup (l1 l2 : Nat) (s : Srt)
+  | tt | ff
 
+def Cell.tm : Cell Srt -> Tm Srt
+  | .clo m s _   => .lam m s
+  | .box l s     => .tup (.ptr l) .null s
+  | .tup l1 l2 s => .tup (.ptr l1) (.ptr l2) s
+  | .tt          => .tt
+  | .ff          => .ff
+
+def Cell.srt : Cell Srt -> Srt
+  | .clo _ s _ => s
+  | .box _ s   => s
+  | .tup _ _ s => s
+  | .tt        => ord.e
+  | .ff        => ord.e
+
+abbrev Heap Srt := Finmap fun (_ : Nat) => Cell Srt
+
+omit ord in
 lemma Heap.fresh (H : Heap Srt) : ∃ l, l ∉ H := by
   generalize e1: H.keys = keys
   cases e2: keys.max with
@@ -20,6 +41,7 @@ lemma Heap.fresh (H : Heap Srt) : ∃ l, l ∉ H := by
     apply keys.not_mem_of_max_lt _ e2
     simp
 
+omit ord in
 lemma Heap.erase_insert {H : Heap Srt} {l v} :
     l ∉ H -> (H.insert l v).erase l = H := by
   intro h
@@ -34,6 +56,7 @@ lemma Heap.erase_insert {H : Heap Srt} {l v} :
     rw [Finmap.lookup_erase_ne e]
     rw [Finmap.lookup_insert_of_ne _ e]
 
+omit ord in
 lemma Heap.insert_erase {H : Heap Srt} {l v} :
     H.lookup l = some v -> (H.erase l).insert l v = H := by
   intro h
@@ -42,6 +65,7 @@ lemma Heap.insert_erase {H : Heap Srt} {l v} :
   | isTrue => subst_vars; simp[h]
   | isFalse ne => simp[ne]
 
+omit ord in
 lemma Heap.erase_insert_comm {H : Heap Srt} {l1 l2 x} :
     l1 ≠ l2 -> (H.insert l1 x).erase l2 = (H.erase l2).insert l1 x := by
   intro ne
@@ -63,6 +87,7 @@ lemma Heap.erase_insert_comm {H : Heap Srt} {l1 l2 x} :
       rw[Finmap.lookup_erase_ne dec2]
       rw[Finmap.lookup_insert_of_ne _ dec1]
 
+omit ord in
 lemma Heap.insert_id {H : Heap Srt} {l t} :
     H.lookup l = some t -> H.insert l t = H := by
   intro h
@@ -71,28 +96,17 @@ lemma Heap.insert_id {H : Heap Srt} {l t} :
   | isTrue => subst_vars; simp[h]
   | isFalse ne => simp[ne]
 
-variable [ord : SrtOrder Srt]
-
 def Weaken (H : Heap Srt) : Prop :=
   ∀ l,
     match H.lookup l with
-    | some (_, s) => s ∈ ord.weaken_set
+    | some m => m.srt ∈ ord.weaken_set
     | none => True
 
 def Contra (H : Heap Srt) : Prop :=
   ∀ l,
     match H.lookup l with
-    | some (_, s) => s ∈ ord.contra_set
+    | some m => m.srt ∈ ord.contra_set
     | none => True
-
--- def HLower (H : Heap Srt) (s0 : Srt) : Prop :=
---   ∀ l,
---     match H.lookup l with
---     | some (_, s) => s ∈ InterSet s0
---     | none => True
-
--- lemma HLower.empty {s : Srt} : HLower ∅ s := by
---   intro l; simp
 
 lemma Weaken.empty : Weaken (∅ : Heap Srt) := by
   intro l; simp
@@ -109,81 +123,35 @@ lemma Contra.union {H1 H2 : Heap Srt} : Contra H1 -> Contra H2 -> Contra (H1 ∪
     simp at heq
     cases heq <;> aesop
 
--- lemma HLower.insert {H : Heap Srt} {l v s s'} :
---     HLower H s -> s' ∈ InterSet s -> HLower (H.insert l (v, s')) s := by
---   intro lw h x
---   cases x.decEq l with
---   | isTrue => subst_vars; simp[h]
---   | isFalse ne => simp[ne]; apply lw
-
-lemma Weaken.insert {H : Heap Srt} {l v s} :
-    Weaken H -> s ∈ ord.weaken_set -> Weaken (H.insert l (v, s)) := by
-  intro lw h x
+lemma Weaken.insert {H : Heap Srt} {l m s} :
+    Weaken H -> s ∈ ord.weaken_set -> m.srt = s -> Weaken (H.insert l m) := by
+  intro wk h e x
   cases x.decEq l with
-  | isTrue => subst_vars; simp[h]
-  | isFalse ne => simp[ne]; apply lw
+  | isTrue =>
+    subst_vars
+    cases m <;> simp_all
+  | isFalse ne => simp[ne]; apply wk
 
-lemma Contra.insert {H : Heap Srt} {l v s} :
-    Contra H -> s ∈ ord.contra_set -> Contra (H.insert l (v, s)) := by
-  intro lw h x
+lemma Contra.insert {H : Heap Srt} {l m s} :
+    Contra H -> s ∈ ord.contra_set -> m.srt = s -> Contra (H.insert l m) := by
+  intro ct h e x
   cases x.decEq l with
-  | isTrue => subst_vars; simp[h]
-  | isFalse ne => simp[ne]; apply lw
+  | isTrue =>
+    subst_vars
+    cases m <;> simp_all
+  | isFalse ne => simp[ne]; apply ct
 
--- lemma HLower.invert {H : Heap Srt} {l v s s'} :
---     HLower (H.insert l (v, s')) s -> s' ∈ InterSet s := by
---   intro lw
---   replace lw := lw l
---   simp at lw; assumption
+lemma Weaken.invert {H : Heap Srt} {l m} :
+    Weaken (H.insert l m) -> m.srt ∈ ord.weaken_set := by
+  intro wk
+  replace wk := wk l
+  simp at wk; assumption
 
-lemma Weaken.invert {H : Heap Srt} {l v s} :
-    Weaken (H.insert l (v, s)) -> s ∈ ord.weaken_set := by
-  intro lw
-  replace lw := lw l
-  simp at lw; assumption
-
-lemma Contra.invert {H : Heap Srt} {l v s} :
-    Contra (H.insert l (v, s)) -> s ∈ ord.contra_set := by
-  intro lw
-  replace lw := lw l
-  simp at lw; assumption
-
--- lemma HLower.cover {H : Heap Srt} {s1 s2 : Srt} :
---     HLower H s1 -> s1 ∈ InterSet s2 -> HLower H s2 := by
---   intro lw h x
---   replace lw := lw x
---   split at lw <;> try simp
---   apply InterSet.trans h lw
-
--- lemma HLower.weaken {H : Heap Srt} {s1 s2 : Srt} :
---     HLower H s1 -> s1 ≤ s2 -> HLower H s2 := by
---   intro lw h
---   apply lw.cover (InterSet.lower_mem h)
-
--- lemma HLower.insert_lower {H} {m : Tm Srt} {l s1 s2} :
---     HLower H s2 -> s1 ≤ s2 ->  HLower (H.insert l (m, s1)) s2 := by
---   intro h lw x
---   split <;> try simp
---   case h_1 opt m1 s3 e =>
---     cases x.decEq l with
---     | isTrue =>
---       subst_vars
---       rw[Finmap.lookup_insert] at e; cases e
---       apply InterSet.lower_mem lw
---     | isFalse ne =>
---       rw[Finmap.lookup_insert_of_ne _ ne] at e
---       replace h := h x
---       simp_rw[e] at h
---       assumption
-
--- lemma HLower.erase_lower {H : Heap Srt} {s} l :
---     HLower H s -> HLower (H.erase l) s := by
---   intro lw x
---   cases x.decEq l with
---   | isTrue => aesop
---   | isFalse ne =>
---     rw[Finmap.lookup_erase_ne ne]
---     apply lw
+lemma Contra.invert {H : Heap Srt} {l m} :
+    Contra (H.insert l m) -> m.srt ∈ ord.contra_set := by
+  intro ct
+  replace ct := ct l
+  simp at ct; assumption
 
 lemma Weaken.erase {H : Heap Srt} l :
     Weaken H -> Weaken (H.erase l) := by
@@ -203,58 +171,24 @@ lemma Contra.erase {H : Heap Srt} l :
     rw[Finmap.lookup_erase_ne ne]
     apply ct
 
--- lemma HLower.union {H1 H2 : Heap Srt} {s1 s2 : Srt} :
---     HLower H1 s1 ->
---     HLower H2 s2 ->
---     s1 ≤ s2 ->
---     HLower (H1 ∪ H2) s2 := by
---   intro lw1 lw2 lw x
---   split <;> try simp
---   case h_1 opt m s h =>
---     rw[Finmap.mem_lookup_union'] at h
---     match h with
---     | .inl h =>
---       simp at h
---       replace lw1 := lw1 x
---       simp_rw[h] at lw1
---       apply InterSet.lower_subset lw lw1
---     | .inr ⟨_, h⟩ =>
---       simp at h
---       replace lw2 := lw2 x
---       simp_rw[h] at lw2
---       assumption
-
 def HMerge (H1 H2 H3 : Heap Srt) : Prop :=
   ∀ l,
     match H1.lookup l, H2.lookup l, H3.lookup l with
-    | some (m1, s1), some (m2, s2), some (m3, s3) =>
-      s1 ∈ ord.contra_set ∧
-      s1 = s2 ∧ s2 = s3 ∧
-      m1 = m2 ∧ m2 = m3
-    | some (m1, s1), none, some (m3, s3) =>
-      s1 ∉ ord.contra_set ∧
-      m1 = m3 ∧ s1 = s3
-    | none, some (m2, s2), some (m3, s3) =>
-      s2 ∉ ord.contra_set ∧
-      m2 = m3 ∧ s2 = s3
+    | some m1, some m2, some m3 =>
+      m3.srt ∈ ord.contra_set ∧ m1 = m2 ∧ m2 = m3
+    | some m1, none, some m3 =>
+      m3.srt ∉ ord.contra_set ∧ m1 = m3
+    | none, some m2, some m3 =>
+      m3.srt ∉ ord.contra_set ∧ m2 = m3
     | none, none, none => True
     | _, _, _ => False
 
--- lemma HLower.merge_refl {H : Heap Srt} : HMerge H H H := by
---   intro lw1 h x
---   replace lw1 := lw1 x
---   split at lw1
---   case h_1 opt m s e =>
---     rw[e]; simp
---     apply InterSet.contra lw1 h
---   case h_2 => aesop
-
 lemma Contra.merge_refl {H : Heap Srt} :
     Contra H -> HMerge H H H := by
-  intro lw1 x
-  replace lw1 := lw1 x
-  split at lw1
-  case h_1 opt m s e =>
+  intro ct1 x
+  replace ct1 := ct1 x
+  split at ct1
+  case h_1 opt m e =>
     rw[e]; simp; assumption
   case h_2 => aesop
 
@@ -264,15 +198,6 @@ lemma HMerge.sym {H1 H2 H3 : Heap Srt} :
   replace mrg := mrg x
   split at mrg <;> aesop
 
--- lemma HMerge.empty {H : Heap Srt} : HMerge H ∅ H := by
---   intro l; split <;> try simp_all
---   case h_5 h1 h2 =>
---     revert h1 h2
---     generalize Finmap.lookup l H = opt
---     cases opt
---     . simp
---     . aesop
-
 lemma HMerge.empty_inv {H1 H2 : Heap Srt} : HMerge H1 ∅ H2 -> H1 = H2 := by
   intro mrg
   apply Finmap.ext_lookup
@@ -280,67 +205,46 @@ lemma HMerge.empty_inv {H1 H2 : Heap Srt} : HMerge H1 ∅ H2 -> H1 = H2 := by
   replace mrg := mrg l; split at mrg
   all_goals aesop
 
--- lemma HMerge.lower_image {H1 H2 H3 : Heap Srt} {s} :
---     HMerge H1 H2 H3 -> HLower H1 s -> HLower H2 s -> HLower H3 s := by
---   intro mrg lw1 lw2 x
---   split <;> try simp
---   case h_1 opt m s h =>
---     replace mrg := mrg x
---     simp_rw[h] at mrg
---     split at mrg <;> try trivial
---     case h_1 h1 h2 e =>
---       cases e; have ⟨_, e1, e2, e3, e4⟩ := mrg; subst_vars
---       replace lw1 := lw1 x; simp_rw[h1] at lw1
---       assumption
---     case h_2 h1 h2 e =>
---       cases e; have ⟨_, e1, e2⟩ := mrg; subst_vars
---       replace lw1 := lw1 x; simp_rw[h1] at lw1
---       assumption
---     case h_3 h1 h2 e =>
---       cases e; have ⟨_, e1, e2⟩ := mrg; subst_vars
---       replace lw2 := lw2 x; simp_rw[h2] at lw2
---       assumption
-
 lemma HMerge.weaken_image {H1 H2 H3 : Heap Srt} :
     HMerge H1 H2 H3 -> Weaken H1 -> Weaken H2 -> Weaken H3 := by
-  intro mrg lw1 lw2 x
+  intro mrg wk1 wk2 x
   split <;> try simp
-  case h_1 opt m s h =>
+  case h_1 opt m h =>
     replace mrg := mrg x
     simp_rw[h] at mrg
     split at mrg <;> try trivial
     case h_1 h1 h2 e =>
-      cases e; have ⟨_, e1, e2, e3, e4⟩ := mrg; subst_vars
-      replace lw1 := lw1 x; simp_rw[h1] at lw1
+      cases e; have ⟨_, e1, e2⟩ := mrg; subst_vars
+      replace wk1 := wk1 x; simp_rw[h1] at wk1
       assumption
     case h_2 h1 h2 e =>
-      cases e; have ⟨_, e1, e2⟩ := mrg; subst_vars
-      replace lw1 := lw1 x; simp_rw[h1] at lw1
+      cases e; have ⟨_, e1⟩ := mrg; subst_vars
+      replace wk1 := wk1 x; simp_rw[h1] at wk1
       assumption
     case h_3 h1 h2 e =>
-      cases e; have ⟨_, e1, e2⟩ := mrg; subst_vars
-      replace lw2 := lw2 x; simp_rw[h2] at lw2
+      cases e; have ⟨_, e1⟩ := mrg; subst_vars
+      replace wk2 := wk2 x; simp_rw[h2] at wk2
       assumption
 
 lemma HMerge.contra_image {H1 H2 H3 : Heap Srt} :
     HMerge H1 H2 H3 -> Contra H1 -> Contra H2 -> Contra H3 := by
-  intro mrg lw1 lw2 x
+  intro mrg ct1 ct2 x
   split <;> try simp
-  case h_1 opt m s h =>
+  case h_1 opt m h =>
     replace mrg := mrg x
     simp_rw[h] at mrg
     split at mrg <;> try trivial
     case h_1 h1 h2 e =>
-      cases e; have ⟨_, e1, e2, e3, e4⟩ := mrg; subst_vars
-      replace lw1 := lw1 x; simp_rw[h1] at lw1
+      cases e; have ⟨_, e1, e2⟩ := mrg; subst_vars
+      replace ct1 := ct1 x; simp_rw[h1] at ct1
       assumption
     case h_2 h1 h2 e =>
-      cases e; have ⟨_, e1, e2⟩ := mrg; subst_vars
-      replace lw1 := lw1 x; simp_rw[h1] at lw1
+      cases e; have ⟨_, e1⟩ := mrg; subst_vars
+      replace ct1 := ct1 x; simp_rw[h1] at ct1
       assumption
     case h_3 h1 h2 e =>
-      cases e; have ⟨_, e1, e2⟩ := mrg; subst_vars
-      replace lw2 := lw2 x; simp_rw[h2] at lw2
+      cases e; have ⟨_, e1⟩ := mrg; subst_vars
+      replace ct2 := ct2 x; simp_rw[h2] at ct2
       assumption
 
 lemma HMerge.split_weaken_hyp {H1 H2 H3 : Heap Srt} {s} :
@@ -385,9 +289,6 @@ lemma HMerge.split_contra' {H1 H2 H3 : Heap Srt} :
     HMerge H1 H2 H3 -> Contra H3 -> Contra H1 := by
   intro mrg wr l
   replace mrg := mrg l; split at mrg <;> try (solve|aesop)
-  -- case h_1 h1 h2 h3 =>
-  --   replace wr := wr l
-  --   rw[h3] at wr; simp_all
   case h_2 h1 h2 h3 =>
     replace wr := wr l
     rw[h3] at wr; simp_all
@@ -407,13 +308,13 @@ lemma HMerge.split_none {H1 H2 H3 : Heap Srt} {l} :
   cases h with
   | inl h1 =>
     rw[Finmap.mem_iff] at h1
-    replace ⟨⟨m, s⟩, h1⟩ := h1
+    replace ⟨m, h1⟩ := h1
     rw[<-Finmap.lookup_eq_none] at h3
     replace mrg := mrg l
     simp_rw[h1,h3] at mrg
     split at mrg <;> try trivial
   | inr h2 =>
-    rw[Finmap.mem_iff] at h2; replace ⟨⟨m, s⟩, h2⟩ := h2
+    rw[Finmap.mem_iff] at h2; replace ⟨m, h2⟩ := h2
     rw[<-Finmap.lookup_eq_none] at h3
     replace mrg := mrg l
     simp_rw[h2,h3] at mrg
@@ -423,7 +324,7 @@ lemma HMerge.mem_left {H1 H2 H3 : Heap Srt} {l} :
     HMerge H1 H2 H3 -> l ∈ H1 -> l ∈ H3 := by
   intro mrg h1
   rw[Finmap.mem_iff] at h1
-  replace ⟨⟨m, s⟩, h1⟩ := h1
+  replace ⟨m, h1⟩ := h1
   replace mrg := mrg l; rw[h1] at mrg
   split at mrg <;> try trivial
   . apply Finmap.mem_of_lookup_eq_some
@@ -431,9 +332,9 @@ lemma HMerge.mem_left {H1 H2 H3 : Heap Srt} {l} :
   . apply Finmap.mem_of_lookup_eq_some
     assumption
 
-lemma HMerge.insert_contra {H1 H2 H3 : Heap Srt} {m l s} :
-    HMerge H1 H2 H3 -> s ∈ ord.contra_set ->
-    HMerge (H1.insert l ⟨m, s⟩) (H2.insert l ⟨m, s⟩) (H3.insert l ⟨m, s⟩) := by
+lemma HMerge.insert_contra {H1 H2 H3 : Heap Srt} {l m} :
+    HMerge H1 H2 H3 -> m.srt ∈ ord.contra_set ->
+    HMerge (H1.insert l m) (H2.insert l m) (H3.insert l m) := by
   intro mrg h x
   cases x.decEq l with
   | isTrue =>
@@ -452,30 +353,26 @@ lemma HMerge.union_contra {H0 H1 H2 H3 : Heap Srt} :
   if h: x ∈ H3 then
     have h0 := h
     rw[Finmap.mem_iff] at h
-    rcases h with ⟨⟨m, s⟩, h⟩
-    if s ∈ ord.contra_set then
+    rcases h with ⟨m, h⟩
+    if m.srt ∈ ord.contra_set then
       replace mrg := mrg x; rw[h] at mrg
       split at mrg <;> try simp_all
       case h_1 heq1 heq2 heq3 =>
         rw[Finmap.lookup_union_left]
         rw[Finmap.lookup_union_left]
-        simp[heq1,heq2]
-        assumption
+        simp[heq1,heq2,mrg]
         rw[Finmap.mem_iff]; aesop
         rw[Finmap.mem_iff]; aesop
-      case h_2 => aesop
-      case h_3 => aesop
     else
       replace mrg := mrg x; rw[h] at mrg
       split at mrg <;> try simp_all
-      case h_1 => aesop
       case h_2 heq1 heq2 heq3 =>
         rw[Finmap.lookup_union_left]
         rw[Finmap.lookup_union_right]
         simp[heq1,heq2]
         have h0 := dsj _ h0
         rw[<-Finmap.lookup_eq_none] at h0
-        simp[h0]; assumption
+        simp[h0,mrg]
         rw[Finmap.mem_iff]; aesop
         rw[Finmap.mem_iff]; aesop
       case h_3 heq1 heq2 =>
@@ -484,7 +381,7 @@ lemma HMerge.union_contra {H0 H1 H2 H3 : Heap Srt} :
         simp[heq1,heq2]
         have h0 := dsj _ h0
         rw[<-Finmap.lookup_eq_none] at h0
-        simp[h0]; assumption
+        simp[h0,mrg]
         rw[Finmap.mem_iff]; aesop
         rw[Finmap.mem_iff]; aesop
   else
@@ -494,15 +391,15 @@ lemma HMerge.union_contra {H0 H1 H2 H3 : Heap Srt} :
     rw[Finmap.lookup_union_right h]
     apply ct.merge_refl
 
-lemma HMerge.insert_lookup {H1 H2 H3 : Heap Srt} {m l s} :
-    HMerge (H1.insert l (m, s)) H2 H3 -> H3.lookup l = some (m, s) := by
+lemma HMerge.insert_lookup {H1 H2 H3 : Heap Srt} {l m} :
+    HMerge (H1.insert l m) H2 H3 -> H3.lookup l = m := by
   intro mrg
   replace mrg := mrg l
   split at mrg <;> simp_all
 
-lemma HMerge.insert_left {H1 H2 H3 : Heap Srt} l m s :
-    HMerge H1 H2 H3 -> l ∉ H3 -> s ∉ ord.contra_set ->
-    HMerge (H1.insert l ⟨m, s⟩) H2 (H3.insert l ⟨m, s⟩) := by
+lemma HMerge.insert_left {H1 H2 H3 : Heap Srt} l m :
+    HMerge H1 H2 H3 -> l ∉ H3 -> m.srt ∉ ord.contra_set ->
+    HMerge (H1.insert l m) H2 (H3.insert l m) := by
   intro mrg h1 h2 x
   have ⟨h3, h4⟩ := mrg.split_none h1
   rw [<-Finmap.lookup_eq_none] at h3
@@ -514,15 +411,6 @@ lemma HMerge.insert_left {H1 H2 H3 : Heap Srt} l m s :
   | isFalse ne =>
     simp[Finmap.lookup_insert_of_ne _ ne]
     apply mrg
-
--- lemma HLower.split_lower {H3 : Heap Srt} {s} :
---     HLower H3 s -> s ∈ ord.contra_set ->
---     ∃ H1 H2, HLower H1 s ∧ HLower H2 s ∧ HMerge H1 H2 H3 := by
---   intro lw h
---   existsi H3, H3; and_intros
---   . assumption
---   . assumption
---   . apply lw.merge_refl h
 
 lemma HLower.split_contra {H3 : Heap Srt} :
     Contra H3 ->
@@ -556,11 +444,10 @@ lemma HMerge.exists_self_contra (H : Heap Srt) :
     case IH l hd tl nn ih =>
       rw[<-Finmap.insert_toFinmap]
       rcases ih with ⟨H0, mrg0, ct0⟩
-      rcases hd with ⟨m, s⟩
-      if mm: s ∈ ord.contra_set then
-        existsi H0.insert l (m, s); and_intros
+      if mm: hd.srt ∈ ord.contra_set then
+        existsi H0.insert l hd; and_intros
         apply mrg0.insert_contra mm
-        apply ct0.insert mm
+        apply ct0.insert mm; rfl
       else
         existsi H0; and_intros
         apply mrg0.insert_left <;> assumption
@@ -570,12 +457,12 @@ lemma HMerge.lookup_collision {H1 H2 H3 : Heap Srt} {l} :
     HMerge H1 H2 H3 -> l ∈ H1 -> H1.lookup l = H3.lookup l := by
   intro mrg h
   rw[Finmap.mem_iff] at h
-  have ⟨⟨m, s⟩, e⟩ := h
+  have ⟨m, e⟩ := h
   replace mrg := mrg l
   rw[e] at mrg; split at mrg <;> aesop
 
-lemma HMerge.insert_inv {H1 H2 H3 : Heap Srt} {m l s} :
-    HMerge (H1.insert l (m, s)) H2 H3 -> l ∉ H1 -> l ∉ H2 ->
+lemma HMerge.insert_inv {H1 H2 H3 : Heap Srt} {l m} :
+    HMerge (H1.insert l m) H2 H3 -> l ∉ H1 -> l ∉ H2 ->
     HMerge H1 H2 (H3.erase l) := by
   intro mrg h1 h2
   have h3 := mrg.insert_lookup
@@ -590,8 +477,8 @@ lemma HMerge.insert_inv {H1 H2 H3 : Heap Srt} {m l s} :
     replace mrg := mrg x
     simp[dec] at mrg; assumption
 
-lemma HMerge.erase {H1 H2 H3 : Heap Srt} {m l s} :
-    HMerge (H1.insert l (m, s)) H2 H3 -> l ∉ H1 ->
+lemma HMerge.erase {H1 H2 H3 : Heap Srt} {l m} :
+    HMerge (H1.insert l m) H2 H3 -> l ∉ H1 ->
     HMerge H1 (H2.erase l) (H3.erase l) := by
   intro mrg h x
   rw[<-Finmap.lookup_eq_none] at h
@@ -603,20 +490,19 @@ lemma HMerge.erase {H1 H2 H3 : Heap Srt} {m l s} :
     simp[dec] at mrg
     assumption
 
-lemma HMerge.not_contra_inv {H1 H2 H3 : Heap Srt} {m s} l :
-    HMerge H1 H2 H3 -> H1.lookup l = some (m, s) ->
-    s ∉ ord.contra_set -> l ∉ H2 := by
+lemma HMerge.not_contra_inv {H1 H2 H3 : Heap Srt} {m} l :
+    HMerge H1 H2 H3 -> H1.lookup l = some m ->
+    m.srt ∉ ord.contra_set -> l ∉ H2 := by
   intro mrg e h
   replace mrg := mrg l
   rw[e] at mrg
   split at mrg <;> simp_all
-  . aesop
-  . rw[Finmap.mem_iff]; aesop
+  rw[Finmap.mem_iff]; aesop
 
-lemma HMerge.shift {H1 H2 H3 : Heap Srt} {l m s} :
-    HMerge (Finmap.insert l (m, s) H1) H2 H3 ->
-    l ∉ H1 -> s ∉ ord.contra_set ->
-    HMerge H1 (Finmap.insert l (m, s) H2) H3 := by
+lemma HMerge.shift {H1 H2 H3 : Heap Srt} {l m} :
+    HMerge (Finmap.insert l m H1) H2 H3 ->
+    l ∉ H1 -> m.srt ∉ ord.contra_set ->
+    HMerge H1 (Finmap.insert l m H2) H3 := by
   intro mrg h1 h2 x
   replace mrg := mrg x
   if dec: x = l then
@@ -626,44 +512,8 @@ lemma HMerge.shift {H1 H2 H3 : Heap Srt} {l m s} :
     rw[h1]; revert mrg
     generalize e: Finmap.lookup x H3 = opt
     split <;> try simp_all
-    intros; subst_vars
-    assumption
+    intros; subst_vars; aesop
   else simp_all
-
--- lemma HMerge.compose {H1 H2 H3 Ha Hb Hx Hy : Heap Srt} {s} :
---     HLower Ha s -> s ∈ ord.contra_set ->
---     HMerge Ha Hb H3 ->
---     HMerge Hx Ha H1 ->
---     HMerge Hy Ha H2 ->
---     HMerge Hx Hy Hb ->
---     HMerge H1 H2 H3 := by
---   intro lw h mrg1 mrg2 mrg3 mrg4 x
---   replace lw := lw x
---   replace mrg1 := mrg1 x
---   replace mrg2 := mrg2 x
---   replace mrg3 := mrg3 x
---   replace mrg4 := mrg4 x
---   split at mrg1 <;> simp_all
---   case h_1 =>
---     split at mrg2 <;> simp_all
---     case h_1 => split at mrg3 <;> simp_all; aesop
---     case h_3 => split at mrg3 <;> simp_all; aesop
---   case h_2 =>
---     split at mrg2 <;> simp_all
---     case h_3 =>
---       split at mrg3 <;> simp_all
---       apply InterSet.contra lw h
---   case h_3 =>
---     split at mrg2 <;> simp_all
---     case h_2 =>
---       split at mrg3 <;> simp_all
---       case h_2 =>
---         have ⟨h, _, _, _⟩ := mrg4; subst_vars
---         assumption
---     case h_4 => split at mrg3 <;> simp_all
---   case h_4 =>
---     split at mrg2 <;> simp_all
---     split at mrg3 <;> simp_all
 
 lemma HMerge.split_disjoint' {H0 H1 H2 H3 : Heap Srt} :
     HMerge H1 H2 H3 -> H3.Disjoint H0 -> H1.Disjoint H0 := by
@@ -694,20 +544,7 @@ lemma HMerge.split {H1 H2 H3 Ha Hb : Heap Srt} :
         have h := Finmap.mem_of_lookup_eq_some e
         rw[Finmap.lookup_union_left h]
         rw[e]; aesop
-      case h_2 e _ _ =>
-        have h := Finmap.mem_of_lookup_eq_some e
-        rw[Finmap.lookup_union_left h]
-        rw[e]; aesop
-      case h_3 e _ ne _ _ =>
-        rw[Finmap.lookup_eq_none] at ne
-        have h := Finmap.mem_of_lookup_eq_some e
-        rw[Finmap.lookup_union_right ne]
-        rw[e]; simp; aesop
     . split at mrg2 <;> simp_all
-      case h_1 e _ _ =>
-        have h := Finmap.mem_of_lookup_eq_some e
-        rw[Finmap.lookup_union_left h]
-        rw[e]; simp; aesop
       case h_2 e _ _ =>
         have h := Finmap.mem_of_lookup_eq_some e
         rw[Finmap.lookup_union_left h]
@@ -735,20 +572,7 @@ lemma HMerge.split {H1 H2 H3 Ha Hb : Heap Srt} :
         have h := Finmap.mem_of_lookup_eq_some e
         rw[Finmap.lookup_union_left h]
         rw[e]; aesop
-      case h_2 e _ _ =>
-        have h := Finmap.mem_of_lookup_eq_some e
-        rw[Finmap.lookup_union_left h]
-        rw[e]; simp; aesop
-      case h_3 e _ ne _ _ =>
-        rw[Finmap.lookup_eq_none] at ne
-        have h := Finmap.mem_of_lookup_eq_some e
-        rw[Finmap.lookup_union_right ne]
-        rw[e]; aesop
     . split at mrg2 <;> simp_all
-      case h_1 e _ _ =>
-        have h := Finmap.mem_of_lookup_eq_some e
-        rw[Finmap.lookup_union_left h]
-        rw[e]; aesop
       case h_2 e _ _ =>
         have h := Finmap.mem_of_lookup_eq_some e
         rw[Finmap.lookup_union_left h]
@@ -796,16 +620,16 @@ lemma SubHeap.refl (H : Heap Srt) : SubHeap H H := by
   apply Finmap.disjoint_empty
   simp
 
-lemma SubHeap.insert (H : Heap Srt) l m s :
-    l ∉ H -> s ∈ ord.contra_set -> SubHeap H (H.insert l (m, s)) := by
+lemma SubHeap.insert (H : Heap Srt) l m :
+    l ∉ H -> m.srt ∈ ord.contra_set -> SubHeap H (H.insert l m) := by
   intro h1 h2
-  apply SubHeap.intro (Finmap.singleton l (m, s))
+  apply SubHeap.intro (Finmap.singleton l m)
   . intro x
     if e: x = l then
       subst_vars; simp
       assumption
     else
-      rw[<-Finmap.mem_singleton x l (m, s) (β := fun _ => Tm Srt × Srt)] at e
+      rw[<-Finmap.mem_singleton x l m (β := fun _ => Cell Srt)] at e
       rw[Finmap.mem_iff] at e
       split <;> try aesop
   . rw[Finmap.Disjoint.eq_1]
