SStructTT.lean
@@ -60,3 +60,5 @@ import SStructTT.SStruct.Runtime.Substitution
 import SStructTT.SStruct.Runtime.Step
 import SStructTT.SStruct.Runtime.Preservation0
 import SStructTT.SStruct.Runtime.Preservation1
+import SStructTT.SStruct.Runtime.Preservation2
+import SStructTT.SStruct.Runtime.Preservation
