SStructTT/SStruct/Erasure/Erased.lean
@@ -152,6 +152,88 @@ lemma Erased.drop_merge {Γ} {Δ1 Δ2 Δ3 : Ctx Srt} {A m m' s} :
   have sp := mrg.toSpine lw h
   apply tym.drop_spine sp
 
+lemma Erased.nf {Γ Δ} {m A : SStruct.Tm Srt} {m'} :
+    Γ ;; Δ ⊢ m ▷ m' : A -> m'.NF Γ.length := by
+  intro erm; induction erm
+  all_goals try (solve | aesop)
+  case var wf hs =>
+    replace hs := wf.hasStatic hs
+    apply hs.var_lt_length
+
+lemma Erased.nf_stack {Γ Δ} {m A : SStruct.Tm Srt} {m' i} :
+    Γ ;; Δ ⊢ m ▷ m' : A -> m'.NF i -> Stack Δ i := by
+  intro erm nf; induction erm generalizing i
+  case var hs =>
+    simp at nf
+    apply hs.stack nf
+  case lam_im ihm =>
+    simp at nf
+    have st := ihm nf
+    cases st
+    case nil im =>
+      simp at im
+      constructor
+      apply im
+    case cons => assumption
+  case lam_ex ihm =>
+    simp at nf
+    have st := ihm nf
+    cases st
+    case nil im => simp at im
+    case cons => assumption
+  case app_im ihm => simp at nf; aesop
+  case app_ex mrg _ _ ihm ihn =>
+    simp at nf
+    have ⟨nf1, nf2⟩ := nf
+    replace ihm := ihm nf1
+    replace ihn := ihn nf2
+    apply mrg.stack_image ihm ihn
+  case tup_im ihm => simp at nf; aesop
+  case tup_ex mrg _ _ _ ihm ihn =>
+    simp at nf
+    have ⟨nf1, nf2⟩ := nf
+    replace ihm := ihm nf1
+    replace ihn := ihn nf2
+    apply mrg.stack_image ihm ihn
+  case prj_im mrg _ _ _ ihm ihn =>
+    simp at nf
+    have ⟨nf1, nf2⟩ := nf
+    replace ihm := ihm nf1
+    replace ihn := ihn nf2
+    cases ihn <;> try simp_all
+    case cons ihn =>
+      cases ihn <;> try simp_all
+      apply mrg.stack_image <;> assumption
+  case prj_ex mrg _ _ _ ihm ihn =>
+    simp at nf
+    have ⟨nf1, nf2⟩ := nf
+    replace ihm := ihm nf1
+    replace ihn := ihn nf2
+    cases ihn <;> try simp_all
+    case cons ihn =>
+      cases ihn <;> try simp_all
+      apply mrg.stack_image <;> assumption
+  case tt =>
+    constructor
+    assumption
+  case ff =>
+    constructor
+    assumption
+  case ite mrg _ _ _ _ ihm ihn1 ihn2 =>
+    simp at nf
+    rcases nf with ⟨nf0, nf1, nf2⟩
+    replace ihm := ihm nf0
+    replace ihn1 := ihn1 nf1
+    apply mrg.stack_image ihm ihn1
+  case rw => aesop
+  case drop mrg _ _ _ _ ihm ihn =>
+    simp at nf
+    have ⟨nf1, nf2⟩ := nf
+    replace ihm := ihm nf1
+    replace ihn := ihn nf2
+    apply mrg.stack_image ihm ihn
+  case conv => aesop
+
 end SStruct.Erasure
 
 namespace SStruct.Dynamic
