SStructTT/SStruct/Runtime/Preservation0.lean
@@ -9,14 +9,14 @@ open Dynamic
 variable {Srt : Type} [ord : SrtOrder Srt]
 
 lemma Resolved.preservation0X {H1 H2 H3 H3' : Heap Srt} {a b c c' A} :
-    HMerge H1 H2 H3 -> WR H2 ->
+    HMerge H1 H2 H3 ->
     [] ;; [] ;; H1 ⊢ a ▷ b ◁ c : A -> Step0 (H3, c) (H3', c') ->
     ∃ H1' b',
       HMerge H1' H2 H3' ∧
       [] ;; [] ;; H1' ⊢ a ▷ b' ◁ c' : A ∧ Erasure.Step0 b b' := by
   generalize e1: [] = Γ
   generalize e2: [] = Δ
-  intro mrg0 wr2 ⟨er, rs, wr1⟩ st; induction er generalizing H1 H2 H3 H3' c c'
+  intro mrg0 ⟨er, rs⟩ st; induction er generalizing H1 H2 H3 H3' c c'
   case var hs =>
     subst_vars; cases hs
   case lam_im =>
@@ -32,10 +32,8 @@ lemma Resolved.preservation0X {H1 H2 H3 H3' : Heap Srt} {a b c c' A} :
     case app =>
       cases st
       case app_M mrg rsm rsn mx st =>
-        have ⟨wr1', wr2'⟩ := mrg.split_wr wr1
         have ⟨Hx, mrg1, mrg2⟩ := mrg0.split mrg.sym
-        have wrx := mrg1.merge_wr wr2' wr2
-        have ⟨H1', mx', mrgx, ⟨erx, rsx, wrx⟩, stx⟩ := ih rfl rfl mrg2.sym wrx rsm wr1' st
+        have ⟨H1', mx', mrgx, ⟨erx, rsx⟩, stx⟩ := ih rfl rfl mrg2.sym rsm st
         have ⟨Hx, mrg1, mrg2⟩ := mrgx.sym.split mrg1
         existsi Hx, .app mx' .null; and_intros
         . assumption
@@ -45,11 +43,9 @@ lemma Resolved.preservation0X {H1 H2 H3 H3' : Heap Srt} {a b c c' A} :
             apply mrg1.sym
             assumption
             assumption
-          . apply mrg1.merge_wr wr2' wrx
         . constructor; assumption
       case app_N mrg rsm rsn n0 dpf st =>
-        have ⟨wr1', wr2'⟩ := mrg.split_wr wr1
-        have ⟨lw, e⟩ := rsn.null_inv wr2'; subst e
+        have ⟨_, e⟩ := rsn.null_inv; subst e
         cases st
     case ptr => cases st
   case app_ex m m' n n' s mrg erm ern ihm ihn =>
@@ -57,30 +53,24 @@ lemma Resolved.preservation0X {H1 H2 H3 H3' : Heap Srt} {a b c c' A} :
     case app =>
       cases st
       case app_M mrg rsm rsn mx st =>
-        have ⟨wr1', wr2'⟩ := mrg.split_wr wr1
         have ⟨Hx, mrg1, mrg2⟩ := mrg0.split mrg.sym
-        have wrx := mrg1.merge_wr wr2' wr2
-        have ⟨H1', mx', mrgx, ⟨erx, rsx, wrx⟩, stx⟩ := ihm rfl rfl mrg2.sym wrx rsm wr1' st
+        have ⟨H1', mx', mrgx, ⟨erx, rsx⟩, stx⟩ := ihm rfl rfl mrg2.sym rsm st
         have ⟨Hx, mrg1, mrg2⟩ := mrgx.sym.split mrg1
         existsi Hx, .app mx' n'; and_intros
         . assumption
         . constructor
           . apply Erased.app_ex Merge.nil erx ern
           . apply Resolve.app mrg1.sym rsx rsn
-          . apply mrg1.merge_wr wr2' wrx
         . constructor; assumption
       case app_N mrg rsm rsn nx dpf st =>
-        have ⟨wr1', wr2'⟩ := mrg.split_wr wr1
         have ⟨Hx, mrg1, mrg2⟩ := mrg0.split mrg
-        have wrx := mrg1.merge_wr wr1' wr2
-        have ⟨H1', nx', mrgx, ⟨erx, rsx, wrx⟩, stx⟩ := ihn rfl rfl mrg2.sym wrx rsn wr2' st
+        have ⟨H1', nx', mrgx, ⟨erx, rsx⟩, stx⟩ := ihn rfl rfl mrg2.sym rsn st
         have ⟨Hx, mrg1, mrg2⟩ := mrgx.sym.split mrg1
         existsi Hx, .app m' nx'; and_intros
         . assumption
         . constructor
           . apply Erased.app_ex Merge.nil erm erx
           . apply Resolve.app mrg1 rsm rsx
-          . apply mrg1.merge_wr wr1' wrx
         . constructor; assumption
     case ptr => cases st
   case tup_im m m' n s i ty erm tyn ih =>
@@ -88,10 +78,8 @@ lemma Resolved.preservation0X {H1 H2 H3 H3' : Heap Srt} {a b c c' A} :
     case tup =>
       cases st
       case tup_M mrg rsm rsn mx st =>
-        have ⟨wr1', wr2'⟩ := mrg.split_wr wr1
         have ⟨Hx, mrg1, mrg2⟩ := mrg0.split mrg.sym
-        have wrx := mrg1.merge_wr wr2' wr2
-        have ⟨H1', mx', mrgx, ⟨erx, rsx, wrx⟩, stx⟩ := ih rfl rfl mrg2.sym wrx rsm wr1' st
+        have ⟨H1', mx', mrgx, ⟨erx, rsx⟩, stx⟩ := ih rfl rfl mrg2.sym rsm st
         have ⟨Hx, mrg1, mrg2⟩ := mrgx.sym.split mrg1
         existsi Hx, .tup mx' .null s; and_intros
         . assumption
@@ -101,11 +89,9 @@ lemma Resolved.preservation0X {H1 H2 H3 H3' : Heap Srt} {a b c c' A} :
             apply mrg1.sym
             assumption
             assumption
-          . apply mrg1.merge_wr wr2' wrx
         . constructor; assumption
       case tup_N mrg rsm rsn n0 dpf st =>
-        have ⟨wr1', wr2'⟩ := mrg.split_wr wr1
-        have ⟨lw, e⟩ := rsn.null_inv wr2'; subst e
+        have ⟨_, e⟩ := rsn.null_inv; subst e
         cases st
     case ptr => cases st
   case tup_ex m m' n n' s i mrg ty erm ern ihm ihn =>
@@ -113,30 +99,24 @@ lemma Resolved.preservation0X {H1 H2 H3 H3' : Heap Srt} {a b c c' A} :
     case tup =>
       cases st
       case tup_M mrg rsm rsn mx st =>
-        have ⟨wr1', wr2'⟩ := mrg.split_wr wr1
         have ⟨Hx, mrg1, mrg2⟩ := mrg0.split mrg.sym
-        have wrx := mrg1.merge_wr wr2' wr2
-        have ⟨H1', mx', mrgx, ⟨erx, rsx, wrx⟩, stx⟩ := ihm rfl rfl mrg2.sym wrx rsm wr1' st
+        have ⟨H1', mx', mrgx, ⟨erx, rsx⟩, stx⟩ := ihm rfl rfl mrg2.sym rsm st
         have ⟨Hx, mrg1, mrg2⟩ := mrgx.sym.split mrg1
         existsi Hx, .tup mx' n' s; and_intros
         . assumption
         . constructor
           . apply Erased.tup_ex Merge.nil ty erx ern
           . apply Resolve.tup mrg1.sym rsx rsn
-          . apply mrg1.merge_wr wr2' wrx
         . constructor; assumption
       case tup_N mrg rsm rsn nx dpf st =>
-        have ⟨wr1', wr2'⟩ := mrg.split_wr wr1
         have ⟨Hx, mrg1, mrg2⟩ := mrg0.split mrg
-        have wrx := mrg1.merge_wr wr1' wr2
-        have ⟨H1', nx', mrgx, ⟨erx, rsx, wrx⟩, stx⟩ := ihn rfl rfl mrg2.sym wrx rsn wr2' st
+        have ⟨H1', nx', mrgx, ⟨erx, rsx⟩, stx⟩ := ihn rfl rfl mrg2.sym rsn st
         have ⟨Hx, mrg1, mrg2⟩ := mrgx.sym.split mrg1
         existsi Hx, .tup m' nx' s; and_intros
         . assumption
         . constructor
           . apply Erased.tup_ex Merge.nil ty erm erx
           . apply Resolve.tup mrg1 rsm rsx
-          . apply mrg1.merge_wr wr1' wrx
         . constructor; assumption
     case ptr => cases st
   case prj_im m m' n n' s sA sB sC i mrg tyC erm ern ihm ihn =>
@@ -144,17 +124,14 @@ lemma Resolved.preservation0X {H1 H2 H3 H3' : Heap Srt} {a b c c' A} :
     case prj =>
       cases st
       case prj_M mrg rsm rsn mx st =>
-        have ⟨wr1', wr2'⟩ := mrg.split_wr wr1
         have ⟨Hx, mrg1, mrg2⟩ := mrg0.split mrg.sym
-        have wrx := mrg1.merge_wr wr2' wr2
-        have ⟨H1', mx', mrgx, ⟨erx, rsx, wrx⟩, stx⟩ := ihm rfl rfl mrg2.sym wrx rsm wr1' st
+        have ⟨H1', mx', mrgx, ⟨erx, rsx⟩, stx⟩ := ihm rfl rfl mrg2.sym rsm st
         have ⟨Hx, mrg1, mrg2⟩ := mrgx.sym.split mrg1
         existsi Hx, .prj mx' n'; and_intros
         . assumption
         . constructor
           . apply Erased.prj_im Merge.nil tyC erx ern
           . apply Resolve.prj mrg1.sym rsx rsn
-          . apply mrg1.merge_wr wr2' wrx
         . constructor; assumption
     case ptr => cases st
   case prj_ex m m' n n' s sA sB sC i mrg tyC erm ern ihm ihn =>
@@ -162,17 +139,14 @@ lemma Resolved.preservation0X {H1 H2 H3 H3' : Heap Srt} {a b c c' A} :
     case prj =>
       cases st
       case prj_M mrg rsm rsn mx st =>
-        have ⟨wr1', wr2'⟩ := mrg.split_wr wr1
         have ⟨Hx, mrg1, mrg2⟩ := mrg0.split mrg.sym
-        have wrx := mrg1.merge_wr wr2' wr2
-        have ⟨H1', mx', mrgx, ⟨erx, rsx, wrx⟩, stx⟩ := ihm rfl rfl mrg2.sym wrx rsm wr1' st
+        have ⟨H1', mx', mrgx, ⟨erx, rsx⟩, stx⟩ := ihm rfl rfl mrg2.sym rsm st
         have ⟨Hx, mrg1, mrg2⟩ := mrgx.sym.split mrg1
         existsi Hx, .prj mx' n'; and_intros
         . assumption
         . constructor
           . apply Erased.prj_ex Merge.nil tyC erx ern
           . apply Resolve.prj mrg1.sym rsx rsn
-          . apply mrg1.merge_wr wr2' wrx
         . constructor; assumption
     case ptr => cases st
   case tt => subst_vars; cases rs; cases st; cases st
@@ -182,41 +156,34 @@ lemma Resolved.preservation0X {H1 H2 H3 H3' : Heap Srt} {a b c c' A} :
     case ite =>
       cases st
       case ite_M mrg rsm rsn1 rsn2 mx st =>
-        have ⟨wr1', wr2'⟩ := mrg.split_wr wr1
         have ⟨Hx, mrg1, mrg2⟩ := mrg0.split mrg.sym
-        have wrx := mrg1.merge_wr wr2' wr2
-        have ⟨H1', mx', mrgx, ⟨erx, rsx, wrx⟩, stx⟩ := ihm rfl rfl mrg2.sym wrx rsm wr1' st
+        have ⟨H1', mx', mrgx, ⟨erx, rsx⟩, stx⟩ := ihm rfl rfl mrg2.sym rsm st
         have ⟨Hx, mrg1, mrg2⟩ := mrgx.sym.split mrg1
         existsi Hx, .ite mx' n1' n2'; and_intros
         . assumption
         . constructor
           . apply Erased.ite Merge.nil tyA erx ern1 ern2
           . apply Resolve.ite mrg1.sym rsx rsn1 rsn2
-          . apply mrg1.merge_wr wr2' wrx
         . constructor; assumption
     case ptr => cases st
   case rw ih =>
     subst_vars
-    replace ih := ih rfl rfl mrg0 wr2 rs wr1 st
-    rcases ih with ⟨H1', b', mrg', ⟨er', rs', wr'⟩, st⟩
+    replace ih := ih rfl rfl mrg0 rs st
+    rcases ih with ⟨H1', b', mrg', ⟨er', rs'⟩, st⟩
     existsi H1', b'; and_intros
     . assumption
     . constructor
       . constructor <;> assumption
-      . assumption
       . assumption
     . assumption
   case drop m m' n n' A B s mrg lw h erm ern ihm ihn =>
     subst_vars; cases mrg; cases rs
     case drop H1' H2' m m' h1 mrg1 rsm rsn =>
       cases st; case drop_elim dp =>
-      have wr3 := mrg0.merge_wr wr1 wr2
-      have wr3' := dp.wr_image wr3
       have ⟨H0, mrg1, mrg2⟩ := mrg0.split mrg1.sym
       have ⟨Hx, mrgx, ct⟩ := dp.resolve rsm mrg2.sym
       have ⟨Hy, mrg1', mrg2'⟩ := mrgx.sym.split mrg1
       have rsn := rsn.merge_contra mrg1' ct
-      have ⟨wry, _⟩ := mrg2'.split_wr wr3'
       existsi Hy, n'; and_intros
       . assumption
       . constructor <;> assumption
@@ -224,12 +191,11 @@ lemma Resolved.preservation0X {H1 H2 H3 H3' : Heap Srt} {a b c c' A} :
     case ptr => cases st
   case conv eq erm tyB ih =>
     subst_vars
-    have ⟨Hx, x, mrgx, ⟨erx, rsx, wrx⟩, stx⟩ := ih rfl rfl mrg0 wr2 rs wr1 st
+    have ⟨Hx, x, mrgx, ⟨erx, rsx⟩, stx⟩ := ih rfl rfl mrg0 rs st
     existsi Hx, x; and_intros
     . assumption
     . constructor
       apply Erased.conv eq erx tyB
-      assumption
       assumption
     . assumption
 
@@ -237,10 +203,8 @@ lemma Resolved.preservation0 {H H' : Heap Srt} {a b c c' A} :
     [] ;; [] ;; H ⊢ a ▷ b ◁ c : A -> Step0 (H, c) (H', c') ->
     ∃ b', [] ;; [] ;; H' ⊢ a ▷ b' ◁ c' : A ∧ Erasure.Step0 b b' := by
   intro rs st
-  have ⟨_, _, wr⟩ := rs
   have ⟨H0, mrg, ct⟩ := HMerge.exists_self_contra H
-  have wr0 := mrg.sym.split_wr' wr
-  have ⟨H0', b', mrg', rs'⟩ := rs.preservation0X mrg wr0 st
+  have ⟨H0', b', mrg', rs'⟩ := rs.preservation0X mrg st
   have e := mrg'.self_contra ct; subst e
   existsi b'; simp_all
 
