SStructTT/SStruct/Runtime/Preservation1.lean
@@ -9,428 +9,338 @@ open Dynamic
 variable {Srt : Type} [ord : SrtOrder Srt]
 
 lemma Resolved.preservation1X {H1 H2 H3 H3' : Heap Srt} {a b c c' A} :
-    HMerge H1 H2 H3 -> WR H2 ->
+    HMerge H1 H2 H3 ->
     [] ;; [] ;; H1 ⊢ a ▷ b ◁ c : A -> Step1 (H3, c) (H3', c') ->
     ∃ H1' H2',
-      HMerge H1' H2' H3' ∧ WR H2' ∧ SubHeap H2 H2' ∧
+      HMerge H1' H2' H3' ∧ SubHeap H2 H2' ∧
       [] ;; [] ;; H1' ⊢ a ▷ b ◁ c' : A := by
   generalize e1: [] = Γ
   generalize e2: [] = Δ
-  intro mrg0 wr2 ⟨er, rs, wr1⟩ st; induction er generalizing H1 H2 H3 H3' c c'
+  intro mrg0 ⟨er, rs⟩ st; induction er generalizing H1 H2 H3 H3' c c'
   case var wf hs =>
     subst_vars; cases hs
   case lam_im A B m m' s sA i lw tyA erm ihm =>
     subst_vars; cases rs
     case lam x rsx hyp =>
       cases st
-      case alloc s l h vl =>
+      case alloc_clo l h nf =>
         clear ihm
-        cases vl
         have ⟨h1, h2⟩ := mrg0.split_none h
-        have nfm := erm.nf; simp at nfm
-        have nfx := rsx.nf_preimage wr1 nfm
         if h3: s ∈ ord.contra_set then
           replace ct := hyp h3
-          existsi H1.insert l (x.lam s, s), H2.insert l (x.lam s, s); and_intros
+          existsi H1.insert l (.clo x s nf), H2.insert l (.clo x s nf); and_intros
           . apply mrg0.insert_contra
             assumption
-          . apply wr2.insert_lam nfx
           . apply SubHeap.insert
             simp[<-Finmap.mem_keys,h2]
             assumption
           . constructor
             . apply Erased.lam_im <;> assumption
             . apply Resolve.ptr
-              . unfold HLookup; simp[h3]; and_intros <;> rfl
+              . simp[HLookup]; and_intros
+                . rfl
+                . simp[Cell.srt,h3]; rfl
               . constructor
                 intro; apply ct.insert; assumption
-                apply rsx.insert_contra h3 h1
-            . apply wr1.insert_lam nfx
+                simp[Cell.srt]
+                apply rsx.insert_contra (by aesop) h1
         else
-          existsi H1.insert l (x.lam s, s), H2; and_intros
+          existsi H1.insert l (.clo x s nf), H2; and_intros
           . apply mrg0.insert_left
             assumption
             assumption
-          . assumption
           . apply SubHeap.refl
           . constructor
             . apply Erased.lam_im <;> assumption
             . apply Resolve.ptr
-              pick_goal 2
-              . constructor <;> assumption
-              . unfold HLookup
-                simp[h3,Heap.erase_insert,h1]
-            . apply wr1.insert_lam nfx
-    case ptr =>
-      cases st
-      case alloc vl => cases vl
+              . simp[HLookup]; and_intros
+                . rfl
+                . simp[Cell.srt,h3]; rfl
+              . simp[Heap.erase_insert,h1]
+                constructor <;> assumption
+    case ptr => cases st
   case lam_ex A B m m' s sA i lw tyA erm ihm =>
     subst_vars; cases rs
     case lam x rsx hyp =>
       cases st
-      case alloc s l h vl =>
-        cases vl
+      case alloc_clo l h nf =>
         have ⟨h1, h2⟩ := mrg0.split_none h
-        have nfm := erm.nf; simp at nfm
-        have nfx := rsx.nf_preimage wr1 nfm
         if h3: s ∈ ord.contra_set then
           replace ct := hyp h3
-          existsi H1.insert l (x.lam s, s), H2.insert l (x.lam s, s); and_intros
+          existsi H1.insert l (.clo x s nf), H2.insert l (.clo x s nf); and_intros
           . apply mrg0.insert_contra
             assumption
-          . apply wr2.insert_lam nfx
           . apply SubHeap.insert
             simp[<-Finmap.mem_keys,h2]
             assumption
           . constructor
             . apply Erased.lam_ex <;> assumption
             . apply Resolve.ptr
-              . unfold HLookup; simp[h3]; and_intros <;> rfl
+              . simp[HLookup]; and_intros
+                . rfl
+                . simp[Cell.srt,h3]; rfl
               . constructor
-                intro; apply ct.insert; assumption
-                apply rsx.insert_contra h3 h1
-            . apply wr1.insert_lam nfx
+                intro; apply ct.insert; assumption; rfl
+                apply rsx.insert_contra (by aesop) h1
         else
-          existsi H1.insert l (x.lam s, s), H2; and_intros
+          existsi H1.insert l (.clo x s nf), H2; and_intros
           . apply mrg0.insert_left
             assumption
             assumption
-          . assumption
           . apply SubHeap.refl
           . constructor
             . apply Erased.lam_ex <;> assumption
             . apply Resolve.ptr
-              pick_goal 2
-              . constructor <;> assumption
-              . unfold HLookup
-                simp[h3,Heap.erase_insert,h1]
-            . apply wr1.insert_lam nfx
-    case ptr =>
-      cases st
-      case alloc vl => cases vl
+              . simp[HLookup]; and_intros
+                . rfl
+                . simp[Cell.srt,h3]; rfl
+              . simp[Heap.erase_insert,h1]
+                constructor <;> assumption
+    case ptr => cases st
   case app_im erm tyn ihm =>
     subst_vars; cases rs
     case app mrg1 rsm rsn =>
-      have ⟨wr1', wr2'⟩ := mrg1.split_wr wr1
       cases st
       case app_M st =>
-        have ⟨ct, e⟩ := rsn.null_inv wr2'; subst e
+        have ⟨ct, e⟩ := rsn.null_inv; subst e
         have ⟨Hx, mrg2, mrg3⟩ := mrg0.split mrg1.sym
-        have wrx := mrg2.merge_wr wr2' wr2
-        have ⟨H1', H2', mrg', wr', sb, ⟨erm', rsm', wr⟩⟩ :=
-          ihm rfl rfl mrg3.sym wrx rsm wr1' st
+        have ⟨H1', H2', mrg', sb, ⟨erm', rsm'⟩⟩ := ihm rfl rfl mrg3.sym rsm st
         clear ihm
         have ⟨H1p, H2p, sb1, sb2, mrg2p⟩ := mrg2.split_subheap sb
         have ⟨Hx, mrg1, mrg2⟩ := mrg'.sym.split mrg2p
         existsi Hx, H2p; and_intros
         . assumption
-        . apply mrg2p.sym.split_wr' wr'
         . assumption
         . constructor
           . constructor <;> assumption
           . apply Resolve.app mrg1.sym
             assumption
             apply rsn.subheap sb1
-          . apply mrg2.split_wr' (mrg'.merge_wr wr wr')
       case app_N st =>
         cases rsn
-        case ptr =>
-          cases st
-          case alloc vl => cases vl
-        case null =>
-          cases st
-          case alloc vl => cases vl
-      case alloc vl => cases vl
-    case ptr =>
-      cases st
-      case alloc vl => cases vl
+        case ptr => cases st
+        case null => cases st
+    case ptr => cases st
   case app_ex mrg1 erm ern ihm ihn =>
     subst_vars; cases mrg1; cases rs
     case app mrg2 rsm rsn =>
-      have ⟨wr1', wr2'⟩ := mrg2.split_wr wr1
       cases st
       case app_M st =>
         clear ihn
         have ⟨Hx, mrg2, mrg3⟩ := mrg0.split mrg2.sym
-        have wrx := mrg2.merge_wr wr2' wr2
-        have ⟨H1', H2', mrg', wr', sb, ⟨erm', rsm', wr⟩⟩ :=
-          ihm rfl rfl mrg3.sym wrx rsm wr1' st
+        have ⟨H1', H2', mrg', sb, ⟨erm', rsm'⟩⟩ := ihm rfl rfl mrg3.sym rsm st
         clear ihm
         have ⟨H1p, H2p, sb1, sb2, mrg2p⟩ := mrg2.split_subheap sb
         have ⟨Hy, mrg1, mrg2⟩ := mrg'.sym.split mrg2p
         existsi Hy, H2p; and_intros
         . assumption
-        . apply mrg2p.sym.split_wr' wr'
         . assumption
         . constructor
           . apply Erased.app_ex Merge.nil <;> assumption
           . apply Resolve.app mrg1.sym
             assumption
             apply rsn.subheap sb1
-          . apply mrg2.split_wr' (mrg'.merge_wr wr wr')
       case app_N st =>
         clear ihm
         have ⟨Hx, mrg2, mrg3⟩ := mrg0.split mrg2
-        have wrx := mrg2.merge_wr wr1' wr2
-        have ⟨H1', H2', mrg', wr', sb, ⟨ern', rsn', wr⟩⟩ :=
-          ihn rfl rfl mrg3.sym wrx rsn wr2' st
+        have ⟨H1', H2', mrg', sb, ⟨ern', rsn'⟩⟩ := ihn rfl rfl mrg3.sym rsn st
         clear ihn
         have ⟨H1p, H2p, sb1, sb2, mrg2p⟩ := mrg2.split_subheap sb
         have ⟨Hy, mrg1, mrg2⟩ := mrg'.sym.split mrg2p
         existsi Hy, H2p; and_intros
         . assumption
-        . apply mrg2p.sym.split_wr' wr'
         . assumption
         . constructor
           . apply Erased.app_ex Merge.nil <;> assumption
           . apply Resolve.app mrg1
             apply rsm.subheap sb1
             assumption
-          . apply mrg2.split_wr' (mrg'.merge_wr wr wr')
-      case alloc vl => cases vl
-    case ptr =>
-      cases st
-      case alloc vl => cases vl
+    case ptr => cases st
   case tup_im s i ty erm tyn ihm =>
     subst_vars; cases rs
     case tup mrg1 rsm rsn =>
-      have ⟨wr1', wr2'⟩ := mrg1.split_wr wr1
       cases st
       case tup_M st =>
-        have ⟨ct, e⟩ := rsn.null_inv wr2'; subst e
+        have ⟨ct, e⟩ := rsn.null_inv; subst e
         have ⟨Hx, mrg2, mrg3⟩ := mrg0.split mrg1.sym
-        have wrx := mrg2.merge_wr wr2' wr2
-        have ⟨H1', H2', mrg', wr', sb, ⟨erm', rsm', wr⟩⟩ :=
-          ihm rfl rfl mrg3.sym wrx rsm wr1' st
+        have ⟨H1', H2', mrg', sb, ⟨erm', rsm'⟩⟩ := ihm rfl rfl mrg3.sym rsm st
         clear ihm
         have ⟨H1p, H2p, sb1, sb2, mrg2p⟩ := mrg2.split_subheap sb
         have ⟨Hy, mrg1, mrg2⟩ := mrg'.sym.split mrg2p
         existsi Hy, H2p; and_intros
         . assumption
-        . apply mrg2p.sym.split_wr' wr'
         . assumption
         . constructor
           . apply Erased.tup_im <;> assumption
           . apply Resolve.tup mrg1.sym
             assumption
             apply rsn.subheap sb1
-          . apply mrg2.split_wr' (mrg'.merge_wr wr wr')
       case tup_N st =>
         cases rsn
-        case ptr =>
-          cases st
-          case alloc vl => cases vl
-        case null =>
-          cases st
-          case alloc vl => cases vl
-      case alloc l h vl =>
+        case ptr => cases st
+        case null => cases st
+      case alloc_box l l1 h =>
         have ⟨h1, h2⟩ := mrg0.split_none h
         have ⟨h1', h2'⟩ := mrg1.split_none h1
-        cases vl; case tup l1 np =>
-        cases np
-        case ptr =>
-          have ⟨_, _⟩ := rsn.null_inv wr2'
-          contradiction
-        case null =>
-          if h3: s ∈ ord.contra_set then
-            existsi H1.insert l (.tup (.ptr l1) .null s, s)
-            existsi H2.insert l (.tup (.ptr l1) .null s, s)
-            and_intros
-            . apply mrg0.insert_contra
-              assumption
-            . apply wr2.insert_tup
-              constructor
-            . apply SubHeap.insert
-              simp[<-Finmap.mem_keys,h2]
-              assumption
-            . constructor
-              . apply Erased.tup_im <;> assumption
-              . apply Resolve.ptr
-                . unfold HLookup; simp[h3]; and_intros <;> rfl
-                . apply Resolve.tup (mrg1.insert_contra h3)
-                  apply rsm.insert_contra h3 h1'
-                  apply rsn.insert_contra h3 h2'
-              . apply wr1.insert_tup
-                constructor
-          else
-            existsi H1.insert l (.tup (.ptr l1) .null s, s), H2; and_intros
-            . apply mrg0.insert_left
-              assumption
-              assumption
-            . assumption
-            . apply SubHeap.refl
-            . constructor
-              . apply Erased.tup_im <;> assumption
-              . apply Resolve.ptr
-                . unfold HLookup; simp[h3]; and_intros <;> rfl
-                . simp[Heap.erase_insert,h1]
-                  apply Resolve.tup mrg1 <;> assumption
-              . apply wr1.insert_tup
-                constructor
-    case ptr =>
-      cases st
-      case alloc vl => cases vl
+        if h3: s ∈ ord.contra_set then
+          existsi H1.insert l (.box l1 s)
+          existsi H2.insert l (.box l1 s)
+          and_intros
+          . apply mrg0.insert_contra
+            assumption
+          . apply SubHeap.insert
+            simp[<-Finmap.mem_keys,h2]
+            assumption
+          . constructor
+            . apply Erased.tup_im <;> assumption
+            . apply Resolve.ptr
+              . simp[HLookup]; and_intros
+                . rfl
+                . simp[Cell.srt,h3]; rfl
+              . apply Resolve.tup (mrg1.insert_contra (by aesop))
+                apply rsm.insert_contra (by aesop) h1'
+                apply rsn.insert_contra (by aesop) h2'
+        else
+          existsi H1.insert l (.box l1 s), H2; and_intros
+          . apply mrg0.insert_left
+            assumption
+            assumption
+          . apply SubHeap.refl
+          . constructor
+            . apply Erased.tup_im <;> assumption
+            . apply Resolve.ptr
+              . simp[HLookup]; and_intros
+                . rfl
+                . simp[Cell.srt,h3]; rfl
+              . simp[Heap.erase_insert,h1]
+                apply Resolve.tup mrg1 <;> assumption
+      case alloc_tup =>
+        have ⟨_, e⟩ := rsn.null_inv; cases e
+    case ptr => cases st
   case tup_ex s i mrg1 ty erm ern ihm ihn =>
     subst_vars; cases mrg1; cases rs
     case tup mrg2 rsm rsn =>
-      have ⟨wr1', wr2'⟩ := mrg2.split_wr wr1
       cases st
       case tup_M st =>
         clear ihn
         have ⟨Hx, mrg3, mrg4⟩ := mrg0.split mrg2.sym
-        have wrx := mrg3.merge_wr wr2' wr2
-        have ⟨H1', H2', mrg', wr', sb, ⟨erm', rsm', wr⟩⟩ :=
-          ihm rfl rfl mrg4.sym wrx rsm wr1' st
+        have ⟨H1', H2', mrg', sb, ⟨erm', rsm'⟩⟩ := ihm rfl rfl mrg4.sym rsm st
         clear ihm
         have ⟨H1p, H2p, sb1, sb2, mrg3p⟩ := mrg3.split_subheap sb
         have ⟨Hy, mrg1, mrg2⟩ := mrg'.sym.split mrg3p
         existsi Hy, H2p; and_intros
         . assumption
-        . apply mrg3p.sym.split_wr' wr'
         . assumption
         . constructor
           . apply Erased.tup_ex Merge.nil <;> assumption
           . apply Resolve.tup mrg1.sym
             assumption
             apply rsn.subheap sb1
-          . apply mrg2.split_wr' (mrg'.merge_wr wr wr')
       case tup_N st =>
         clear ihm
         have ⟨Hx, mrg3, mrg4⟩ := mrg0.split mrg2
-        have wrx := mrg3.merge_wr wr1' wr2
-        have ⟨H1', H2', mrg', wr', sb, ⟨ern', rsn', wr⟩⟩ :=
-          ihn rfl rfl mrg4.sym wrx rsn wr2' st
+        have ⟨H1', H2', mrg', sb, ⟨ern', rsn'⟩⟩ := ihn rfl rfl mrg4.sym rsn st
         clear ihn
         have ⟨H1p, H2p, sb1, sb2, mrg3p⟩ := mrg3.split_subheap sb
         have ⟨Hy, mrg1, mrg2⟩ := mrg'.sym.split mrg3p
         existsi Hy, H2p; and_intros
         . assumption
-        . apply mrg3p.sym.split_wr' wr'
         . assumption
         . constructor
           . apply Erased.tup_ex Merge.nil <;> assumption
           . apply Resolve.tup mrg1
             apply rsm.subheap sb1
             assumption
-          . apply mrg2.split_wr' (mrg'.merge_wr wr wr')
-      case alloc vl =>
-        cases vl
-        case tup l h l1 np =>
-          have ⟨h1, h2⟩ := mrg0.split_none h
-          have ⟨h1', h2'⟩ := mrg2.split_none h1
-          cases np
-          case ptr l2 =>
-            if h3: s ∈ ord.contra_set then
-              existsi H1.insert l (.tup (.ptr l1) (.ptr l2) s, s)
-              existsi H2.insert l (.tup (.ptr l1) (.ptr l2) s, s)
-              and_intros
-              . apply mrg0.insert_contra
-                assumption
-              . apply wr2.insert_tup
-                constructor
-              . apply SubHeap.insert
-                simp[<-Finmap.mem_keys,h2]
-                assumption
-              . constructor
-                . apply Erased.tup_ex Merge.nil <;> assumption
-                . apply Resolve.ptr
-                  . unfold HLookup; simp[h3]; and_intros <;> rfl
-                  . apply Resolve.tup (mrg2.insert_contra h3)
-                    apply rsm.insert_contra h3 h1'
-                    apply rsn.insert_contra h3 h2'
-                . apply wr1.insert_tup
-                  constructor
-            else
-              existsi H1.insert l (.tup (.ptr l1) (.ptr l2) s, s), H2; and_intros
-              . apply mrg0.insert_left
-                assumption
-                assumption
-              . assumption
-              . apply SubHeap.refl
-              . constructor
-                . apply Erased.tup_ex Merge.nil <;> assumption
-                . apply Resolve.ptr
-                  . unfold HLookup; simp[h3]; and_intros <;> rfl
-                  . simp[Heap.erase_insert,h1]
-                    apply Resolve.tup mrg2 <;> assumption
-                . apply wr1.insert_tup
-                  constructor
-          case null =>
-            cases rsn
-            exfalso; apply ern.null_preimage
-    case ptr =>
-      cases st
-      case alloc vl => cases vl
+      case alloc_box => sorry
+      case alloc_tup l l1 l2 h =>
+        have ⟨h1, h2⟩ := mrg0.split_none h
+        have ⟨h1', h2'⟩ := mrg2.split_none h1
+        if h3: s ∈ ord.contra_set then
+          existsi H1.insert l (.tup l1 l2 s)
+          existsi H2.insert l (.tup l1 l2 s)
+          and_intros
+          . apply mrg0.insert_contra
+            assumption
+          . apply SubHeap.insert
+            simp[<-Finmap.mem_keys,h2]
+            assumption
+          . constructor
+            . apply Erased.tup_ex Merge.nil <;> assumption
+            . apply Resolve.ptr
+              . simp[HLookup]; and_intros
+                . rfl
+                . simp[Cell.srt,h3]; rfl
+              . apply Resolve.tup (mrg2.insert_contra (by aesop))
+                apply rsm.insert_contra (by aesop) h1'
+                apply rsn.insert_contra (by aesop) h2'
+        else
+          existsi H1.insert l (.tup l1 l2 s), H2; and_intros
+          . apply mrg0.insert_left
+            assumption
+            assumption
+          . apply SubHeap.refl
+          . constructor
+            . apply Erased.tup_ex Merge.nil <;> assumption
+            . apply Resolve.ptr
+              . simp[HLookup]; and_intros
+                . rfl
+                . simp[Cell.srt,h3]; rfl
+              . simp[Heap.erase_insert,h1]
+                apply Resolve.tup mrg2 <;> assumption
+    case ptr => cases st
   case prj_im mrg1 ty erm ern ihm ihn =>
     subst_vars; cases mrg1; cases rs
     case prj mrg2 rsm rsn =>
-      have ⟨wr1', wr2'⟩ := mrg2.split_wr wr1
       cases st
       case prj_M st =>
         clear ihn
         have ⟨Hx, mrg2, mrg3⟩ := mrg0.split mrg2.sym
-        have wrx := mrg2.merge_wr wr2' wr2
-        have ⟨H1', H2', mrg', wr', sb, ⟨erm', rsm', wr⟩⟩ :=
-          ihm rfl rfl mrg3.sym wrx rsm wr1' st
+        have ⟨H1', H2', mrg', sb, ⟨erm', rsm'⟩⟩ := ihm rfl rfl mrg3.sym rsm st
         clear ihm
         have ⟨H1p, H2p, sb1, sb2, mrg2p⟩ := mrg2.split_subheap sb
         have ⟨Hy, mrg1, mrg2⟩ := mrg'.sym.split mrg2p
         existsi Hy, H2p; and_intros
         . assumption
-        . apply mrg2p.sym.split_wr' wr'
         . assumption
         . constructor
           . apply Erased.prj_im Merge.nil <;> assumption
           . apply Resolve.prj mrg1.sym
             assumption
             apply rsn.subheap sb1
-          . apply mrg2.split_wr' (mrg'.merge_wr wr wr')
-      case alloc vl => cases vl
-    case ptr =>
-      cases st
-      case alloc vl => cases vl
+    case ptr => cases st
   case prj_ex mrg1 ty erm ern ihm ihn =>
     subst_vars; cases mrg1; cases rs
     case prj mrg2 rsm rsn =>
-      have ⟨wr1', wr2'⟩ := mrg2.split_wr wr1
       cases st
       case prj_M st =>
         clear ihn
         have ⟨Hx, mrg2, mrg3⟩ := mrg0.split mrg2.sym
-        have wrx := mrg2.merge_wr wr2' wr2
-        have ⟨H1', H2', mrg', wr', sb, ⟨erm', rsm', wr⟩⟩ :=
-          ihm rfl rfl mrg3.sym wrx rsm wr1' st
+        have ⟨H1', H2', mrg', sb, ⟨erm', rsm'⟩⟩ := ihm rfl rfl mrg3.sym rsm st
         clear ihm
         have ⟨H1p, H2p, sb1, sb2, mrg2p⟩ := mrg2.split_subheap sb
         have ⟨Hy, mrg1, mrg2⟩ := mrg'.sym.split mrg2p
         existsi Hy, H2p; and_intros
         . assumption
-        . apply mrg2p.sym.split_wr' wr'
         . assumption
         . constructor
           . apply Erased.prj_ex Merge.nil <;> assumption
           . apply Resolve.prj mrg1.sym
             assumption
             apply rsn.subheap sb1
-          . apply mrg2.split_wr' (mrg'.merge_wr wr wr')
-      case alloc vl => cases vl
-    case ptr =>
-      cases st
-      case alloc vl => cases vl
+    case ptr => cases st
   case tt =>
     subst_vars; cases rs
     case tt ct =>
       cases st
-      case alloc s l h vl =>
-        cases vl
+      case alloc_tt l h =>
         have ⟨h1, h2⟩ := mrg0.split_none h
-        existsi H1.insert l (.tt, ord.e)
-        existsi H2.insert l (.tt, ord.e)
+        existsi H1.insert l .tt
+        existsi H2.insert l .tt
         and_intros
-        . apply mrg0.insert_contra ord.e_contra
-        . apply wr2.insert_tt
-        . apply SubHeap.intro (Finmap.singleton l (.tt, ord.e))
-          apply Contra.empty.insert ord.e_contra
+        . apply mrg0.insert_contra
+          simp[Cell.srt]; apply ord.e_contra
+        . apply SubHeap.intro (Finmap.singleton l .tt)
+          apply Contra.empty.insert ord.e_contra (by aesop)
           rw[Finmap.Disjoint.eq_1]; intros; aesop
           apply Finmap.ext_lookup; intro x
           if e: x = l then
@@ -441,27 +351,25 @@ lemma Resolved.preservation1X {H1 H2 H3 H3' : Heap Srt} {a b c c' A} :
             simp[e]
         . constructor
           . constructor <;> assumption
-          . apply Resolve.ptr (H2 := (Finmap.insert l (Tm.tt, SrtOrder.e) H1))
-            unfold HLookup; simp[ord.e_contra]; rfl
-            constructor; apply ct.insert ord.e_contra
-          . apply wr1.insert_tt
-    case ptr =>
-      cases st
-      case alloc vl => cases vl
+          . apply Resolve.ptr (H2 := H1.insert l .tt)
+            simp[HLookup]; and_intros
+            . rfl
+            . simp[Cell.srt,ord.e_contra]
+            . constructor; apply ct.insert ord.e_contra; rfl
+    case ptr => cases st
   case ff =>
     subst_vars; cases rs
     case ff ct =>
       cases st
-      case alloc s l h vl =>
-        cases vl
+      case alloc_ff l h =>
         have ⟨h1, h2⟩ := mrg0.split_none h
-        existsi H1.insert l (.ff, ord.e)
-        existsi H2.insert l (.ff, ord.e)
+        existsi H1.insert l .ff
+        existsi H2.insert l .ff
         and_intros
-        . apply mrg0.insert_contra ord.e_contra
-        . apply wr2.insert_ff
-        . apply SubHeap.intro (Finmap.singleton l (.ff, ord.e))
-          apply Contra.empty.insert ord.e_contra
+        . apply mrg0.insert_contra
+          simp[Cell.srt]; apply ord.e_contra
+        . apply SubHeap.intro (Finmap.singleton l .ff)
+          apply Contra.empty.insert ord.e_contra (by aesop)
           rw[Finmap.Disjoint.eq_1]; intros; aesop
           apply Finmap.ext_lookup; intro x
           if e: x = l then
@@ -472,30 +380,25 @@ lemma Resolved.preservation1X {H1 H2 H3 H3' : Heap Srt} {a b c c' A} :
             simp[e]
         . constructor
           . constructor <;> assumption
-          . apply Resolve.ptr (H2 := (Finmap.insert l (Tm.ff, SrtOrder.e) H1))
-            unfold HLookup; simp[ord.e_contra]; rfl
-            constructor; apply ct.insert ord.e_contra
-          . apply wr1.insert_ff
-    case ptr =>
-      cases st
-      case alloc vl => cases vl
+          . apply Resolve.ptr (H2 := H1.insert l .ff)
+            simp[HLookup]; and_intros
+            . rfl
+            . simp[Cell.srt,ord.e_contra]
+            . constructor; apply ct.insert ord.e_contra; rfl
+    case ptr => cases st
   case ite mrg1 ty erm ern1 ern2 ihm ihn1 ihn2 =>
     subst_vars; cases mrg1; cases rs
     case ite mrg2 rsm rsn1 rsn2 =>
-      have ⟨wr1', wr2'⟩ := mrg2.split_wr wr1
       cases st
       case ite_M st =>
         clear ihn1 ihn2
         have ⟨Hx, mrg2, mrg3⟩ := mrg0.split mrg2.sym
-        have wrx := mrg2.merge_wr wr2' wr2
-        have ⟨H1', H2', mrg', wr', sb, ⟨erm', rsm', wr⟩⟩ :=
-          ihm rfl rfl mrg3.sym wrx rsm wr1' st
+        have ⟨H1', H2', mrg', sb, ⟨erm', rsm'⟩⟩ := ihm rfl rfl mrg3.sym rsm st
         clear ihm
         have ⟨H1p, H2p, sb1, sb2, mrg2p⟩ := mrg2.split_subheap sb
         have ⟨Hy, mrg1, mrg2⟩ := mrg'.sym.split mrg2p
         existsi Hy, H2p; and_intros
         . assumption
-        . apply mrg2p.sym.split_wr' wr'
         . assumption
         . constructor
           . apply Erased.ite Merge.nil <;> assumption
@@ -503,17 +406,11 @@ lemma Resolved.preservation1X {H1 H2 H3 H3' : Heap Srt} {a b c c' A} :
             assumption
             apply rsn1.subheap sb1
             apply rsn2.subheap sb1
-          . apply mrg2.split_wr' (mrg'.merge_wr wr wr')
-      case alloc vl => cases vl
-    case ptr =>
-      cases st
-      case alloc vl => cases vl
+    case ptr => cases st
   case rw tyA erm tyn ih =>
     subst_vars
-    have ⟨H1', H2', mrg', wr', sb, ⟨erm', rsm', wr⟩⟩ :=
-      ih rfl rfl mrg0 wr2 rs wr1 st
+    have ⟨H1', H2', mrg', sb, ⟨erm', rsm'⟩⟩ := ih rfl rfl mrg0 rs st
     existsi H1', H2'; and_intros
-    . assumption
     . assumption
     . assumption
     . constructor
@@ -521,21 +418,14 @@ lemma Resolved.preservation1X {H1 H2 H3 H3' : Heap Srt} {a b c c' A} :
         assumption
         assumption
       . assumption
-      . assumption
   case drop A B s mrg lw h erm ern ihm ihn =>
     subst_vars; cases mrg; cases rs
-    case drop =>
-      cases st
-      case alloc vl => cases vl
-    case ptr =>
-      cases st
-      case alloc vl => cases vl
+    case drop => cases st
+    case ptr => cases st
   case conv eq erm tyB ih =>
     subst_vars
-    have ⟨H1', H2', mrg', wr', sb, ⟨erm', rsm', wr⟩⟩ :=
-      ih rfl rfl mrg0 wr2 rs wr1 st
+    have ⟨H1', H2', mrg', sb, ⟨erm', rsm'⟩⟩ := ih rfl rfl mrg0 rs st
     existsi H1', H2'; and_intros
-    . assumption
     . assumption
     . assumption
     . constructor
@@ -543,16 +433,13 @@ lemma Resolved.preservation1X {H1 H2 H3 H3' : Heap Srt} {a b c c' A} :
         assumption
         assumption
       . assumption
-      . assumption
 
 lemma Resolved.preservation1 {H1 H2 : Heap Srt} {a b c c' A} :
     [] ;; [] ;; H1 ⊢ a ▷ b ◁ c : A -> Step1 (H1, c) (H2, c') ->
     [] ;; [] ;; H2 ⊢ a ▷ b ◁ c' : A := by
   intro rsm st
   have ⟨H0, mrg, ct⟩ := HMerge.exists_self_contra H1
-  have ⟨_, _, wr⟩ := rsm
-  have wr0 := mrg.sym.split_wr' wr
-  have ⟨H1', H2', mrg', wr', sb, rsm'⟩ := rsm.preservation1X mrg wr0 st
+  have ⟨H1', H2', mrg', sb, rsm'⟩ := rsm.preservation1X mrg st
   have ct := sb.contra_image ct
   have e := mrg'.self_contra ct; subst e
   assumption
